Assorted code cleanup

Gaea/Peano/Props.lean
@@ -6,64 +6,68 @@ import Gaea.Syntax.Logic
 import Gaea.Syntax.Notation
 import Gaea.Logic.Notation
 
+universes u v
+
 open Gaea.Logic
 open Gaea.Syntax
 
 namespace Gaea.Peano.Props
 
-universes u v
-
 -- Axiom 1
-def natZero {P : Sort u} (N : Type u) [Nat P N] [Zero N] : P :=
-  nat (0 : N)
+def natZero {P : Sort u} (T : Type v) [Nat P T] [Zero T] : P :=
+  nat (0 : T)
 
 -- Axiom 2
-def eqNatRefl {P : Sort u} (N : Sort v) 
-  [LForall P N] [LIf P] [LEq P N] [Nat P N] : P :=
-  forall (x : N) => nat x -> x = x
+def eqNatRefl {P : Sort u} (T : Sort v) 
+  [LForall P T] [LIf P] [LEq P T] [Nat P T] : P :=
+  forall (x : T) => nat x -> x = x
 
 -- Axiom 3
-def eqNatSymm {P : Sort u} (N : Sort v) 
-  [LForall P N] [LIf P] [LAnd P] [LEq P N] [Nat P N]: P :=
-  forall (x y : N) => nat x /\ nat y -> (x = y -> y = x)
+def eqNatSymm {P : Sort u} (T : Sort v) 
+  [LForall P T] [LIf P] [LAnd P] [LEq P T] [Nat P T] : P :=
+  forall (x y : T) => nat x /\ nat y -> (x = y -> y = x)
 
 -- Axiom 4
-def eqNatTrans {P : Sort u} (N : Sort v) 
-  [LForall P N] [LIf P] [LAnd P] [LEq P N] [Nat P N] : P :=
-  forall (x y z : N) => nat x /\ nat y /\ nat z -> (x = y /\ y = z -> x = z)
+def eqNatTrans {P : Sort u} (T : Sort v) 
+  [LForall P T] [LIf P] [LAnd P] [LEq P T] [Nat P T] : P :=
+  forall (x y z : T) => nat x /\ nat y /\ nat z -> (x = y /\ y = z -> x = z)
 
 -- Axiom 5
-def natEq {P : Sort u} (L : Logic P) (N : Sort v) 
-  [LForall P N] [LIf P] [LEq P N] [Nat P N] : P :=
-  forall (a b : N) => nat b -> (a = b) -> nat a
+def natEq {P : Sort u} (L : Logic P) (T : Sort v) 
+  [LForall P T] [LIf P] [LAnd P] [LEq P T] [Nat P T] : P :=
+  forall (a b : T) => nat b /\ a = b -> nat a
 
 -- Axiom 6
-def natSuccNat {P : Sort u} (N : Sort v) 
-  [LForall P N] [LIf P] [Nat P N] [Succ N] : P :=
-  forall (n : N) => nat n -> nat (S n)
+def natSuccNat {P : Sort u} (T : Sort v) 
+  [LForall P T] [LIf P] [Nat P T] [Succ T] : P :=
+  forall (n : T) => nat n -> nat (S n)
+
+-- Axiom 7
+def succNatOto {P : Sort u} (T : Sort v) 
+  [LForall P T] [LIf P] [LAnd P] [LIff P] [LEq P T] [Nat P T] [Succ T] : P :=
+  forall (m n : T) => nat m /\ nat n -> (m = n <-> S m = S n)
 
 -- Axiom 7a
-def succNatSubst {P : Sort u} (N : Sort v) 
-  [LForall P N] [LIf P] [LAnd P] [LEq P N] [Nat P N] [Succ N] : P  :=
-  forall (m n : N) => nat m /\ nat n -> (m = n -> S m = S n)
+def succNatSubst {P : Sort u} (T : Sort v) 
+  [LForall P T] [LIf P] [LAnd P] [LEq P T] [Nat P T] [Succ T] : P :=
+  forall (m n : T) => nat m /\ nat n -> (m = n -> S m = S n)
 
 -- Axiom 7b
-def succNatInj {P : Sort u} (N : Sort v) 
-  [LForall P N] [LIf P] [LAnd P] [LEq P N] [Nat P N] [Succ N] : P  :=
-  forall (m n : N) => nat m /\ nat n -> (S m = S n -> m = n)
+def succNatInj {P : Sort u} (T : Sort v) 
+  [LForall P T] [LIf P] [LAnd P] [LEq P T] [Nat P T] [Succ T] : P :=
+  forall (m n : T) => nat m /\ nat n -> (S m = S n -> m = n)
 
 -- Axiom 8
-def succNatEqZeroFalse {P : Sort u} (N : Type v) 
-  [LForall P N] [LIf P] [LAnd P] [LEq P N] [Nat P N] [Zero N] [Succ N] [False P] : P  :=
-  forall (m n : N) => nat m /\ nat n -> (S n = 0 -> false)
+def succNatEqZeroFalse {P : Sort u} (T : Type v) 
+  [LForall P T] [LIf P] [LAnd P] [LEq P T] [False P] [Nat P T] [Zero T] [Succ T] : P :=
+  forall (m n : T) => nat m /\ nat n -> (S n = 0 -> false)
 
 -- Axiom 9
-def natInduction 
-  {P : Sort u} (N : Type v) [Nat P N] 
-  [LForall P (N -> P)] [LForall P N] [LIf P] [LAnd P] [LEq P N] 
-  [Nat P N] [Zero N] [Succ N] : P := 
-  forall (f : N -> P) => 
-    f 0 -> (forall (n : N) => nat n -> (f n -> f (S n))) ->
-      forall (n : N) => nat n -> f n
+def natInduction {P : Sort u} (T : Type v) 
+  [LForall P (T -> P)] [LForall P T] [LIf P] [LAnd P] [LEq P T] 
+  [Nat P T] [Zero T] [Succ T] : P := 
+  forall (f : T -> P) => 
+    f 0 -> (forall (n : T) => nat n -> (f n -> f (S n))) ->
+      forall (n : T) => nat n -> f n
 
 end Gaea.Peano.Props
