Gaea/Peano/Rules.lean
@@ -6,92 +6,105 @@ import Gaea.Syntax.Logic
 import Gaea.Syntax.Notation
 import Gaea.Logic.Notation
 
+universes u v w
+
 open Gaea.Logic
 open Gaea.Syntax
 
 namespace Gaea.Peano.Rules
 
-universes u v w
-
+--------------------------------------------------------------------------------
 -- Natural Axioms
+--------------------------------------------------------------------------------
 
 -- Axiom 1
-def NatZero {P : Sort u} (L : Logic P) (N : Type v) [Zero N] [Nat P N] :=
-  L |- nat (0 : N)
+def NatZero {P : Sort u} (L : Logic P) (T : Type v) [Zero T] [Nat P T] :=
+  L |- nat (0 : T)
 
 -- Axiom 2
-def EqNatRefl {P : Sort u} (L : Logic P) (N : Sort v) [Nat P N] [LEq P N] :=
-  (x : N) -> (L |- nat x) -> (L |- x = x)
+def EqNatRefl {P : Sort u} (L : Logic P) (T : Sort v) [Nat P T] [LEq P T] :=
+  (x : T) -> (L |- nat x) -> (L |- x = x)
 
 -- Axiom 3
-def EqNatSymm {P : Sort u} (L : Logic P) (N : Sort v) [Nat P N] [LEq P N] :=
-  (x y : N) -> (L |- nat x) -> (L |- nat y) ->
+def EqNatSymm {P : Sort u} (L : Logic P) (T : Sort v) [Nat P T] [LEq P T] :=
+  (x y : T) -> (L |- nat x) -> (L |- nat y) ->
     (L |- x = y) -> (L |- y = x)
 
 -- Axiom 4
-def EqNatTrans {P : Sort u} (L : Logic P) (N : Sort v) [Nat P N] [LEq P N] :=
-  (x y z : N) -> (L |- nat x) -> (L |- nat y) -> (L |- nat z) -> 
+def EqNatTrans {P : Sort u} (L : Logic P) (T : Sort v) [Nat P T] [LEq P T] :=
+  (x y z : T) -> (L |- nat x) -> (L |- nat y) -> (L |- nat z) -> 
     (L |- x = y) -> (L |- y = z) -> (L |- x = z)
 
 -- Axiom 5
-def NatEq {P : Sort u} (L : Logic P) (N : Sort v) [Nat P N] [LEq P N] :=
-  (a b : N) -> (L |- nat b) -> (L |- a = b) -> (L |- nat a)
+def NatEq {P : Sort u} (L : Logic P) (T : Sort v) [Nat P T] [LEq P T] :=
+  (a b : T) -> (L |- nat b) -> (L |- a = b) -> (L |- nat a)
 
 -- Axiom 6
-def NatSuccNat {P : Sort u} (L : Logic P) (N : Sort v) [Nat P N] [Succ N]:=
-  (n : N) -> (L |- nat n) -> (L |- nat (S n))
+def NatSuccNat {P : Sort u} (L : Logic P) (T : Sort v) [Nat P T] [Succ T]:=
+  (n : T) -> (L |- nat n) -> (L |- nat (S n))
 
 -- Axiom 7a
 def SuccNatSubst 
-  {P : Sort u} (L : Logic P) (N : Sort v) [Nat P N] [LEq P N] [Succ N]  :=
-  (m n : N) -> (L |- nat m) -> (L |- nat n)-> 
+  {P : Sort u} (L : Logic P) (T : Sort v) [Nat P T] [LEq P T] [Succ T]  :=
+  (m n : T) -> (L |- nat m) -> (L |- nat n) -> 
     (L |- m = n) -> (L |- S m = S n)
 
 -- Axiom 7b
 def SuccNatInj 
-  {P : Sort u} (L : Logic P) (N : Sort v) [Nat P N] [LEq P N] [Succ N] :=
-  (m n : N) -> (L |- nat m) -> (L |- nat n) -> 
+  {P : Sort u} (L : Logic P) (T : Sort v) [Nat P T] [LEq P T] [Succ T] :=
+  (m n : T) -> (L |- nat m) -> (L |- nat n) -> 
     (L |- S m = S n) -> (L |- m = n)
 
 -- Axiom 8
 def SuccNatEqZeroFalse 
-  {P : Sort u} (L : Logic P) (N : Type v) 
-  [Nat P N] [LEq P N] [Succ N] [Zero N] [False P] :=
-  (m n : N) -> (L |- nat m) -> (L |- nat n) -> 
+  {P : Sort u} (L : Logic P) (T : Type v) 
+  [Nat P T] [LEq P T] [Succ T] [Zero T] [False P] :=
+  (m n : T) -> (L |- nat m) -> (L |- nat n) -> 
     (L |- S n = 0) -> (L |- false)
 
 -- Axiom 9
+-- Induction over predicates
 def NatInduction 
-  {P : Sort u} (L : Logic P) (N : Type v) [Nat P N] [Zero N] [Succ N] := 
-  (f : N -> P) -> (L |- f 0) -> 
-  ((n : N) -> (L |- nat n) -> (L |- f n) -> (L |- f (S n))) ->
-  ((n : N) -> (L |- nat n) -> (L |- f n))
+  {P : Sort u} (L : Logic P) (T : Type v) [Nat P T] [Zero T] [Succ T] := 
+  (f : T -> P) -> (L |- f 0) -> 
+  ((n : T) -> (L |- nat n) -> (L |- f n) -> (L |- f (S n))) ->
+  ((n : T) -> (L |- nat n) -> (L |- f n))
 
+-- Axiom 9 (Alt)
+-- Induction over schemas
 def NatInduction'
-  {P : Sort u} (L : Logic P) (N : Type v) [Nat P N] [Zero N] [Succ N] := 
-  (f : N -> Sort w) -> f 0 ->
-  ((n : N) -> (L |- nat n) -> (f n -> f (S n))) ->
-  ((n : N) -> (L |- nat n) -> f n)
+  {P : Sort u} (L : Logic P) (T : Type v) [Nat P T] [Zero T] [Succ T] := 
+  (f : T -> Sort w) -> f 0 ->
+  ((n : T) -> (L |- nat n) -> (f n -> f (S n))) ->
+  ((n : T) -> (L |- nat n) -> f n)
 
+--------------------------------------------------------------------------------
 -- Addition Axioms
+--------------------------------------------------------------------------------
 
+-- Axiom 1
 def AddNatZeroEqNat 
-  {P : Sort u} (L : Logic P) (N : Type v) [LEq P N] [Nat P N] [Zero N] [Add N] :=
-  (a : N) -> (L |- nat a) -> (L |- a + 0 = a)
+  {P : Sort u} (L : Logic P) (T : Type v) [LEq P T] [Nat P T] [Zero T] [Add T] :=
+  (a : T) -> (L |- nat a) -> (L |- a + 0 = a)
 
+-- Axiom 2
 def AddNatSuccEqSucc 
-  {P : Sort u} (L : Logic P) (N : Type v) [LEq P N] [Nat P N] [Succ N] [Add N] := 
-  (a b : N) -> (L |- nat a) -> (L |- nat b) -> (L |- a + S b = S (a + b))
+  {P : Sort u} (L : Logic P) (T : Type v) [LEq P T] [Nat P T] [Succ T] [Add T] := 
+  (a b : T) -> (L |- nat a) -> (L |- nat b) -> (L |- a + S b = S (a + b))
 
+--------------------------------------------------------------------------------
 -- Multiplication Axioms
+--------------------------------------------------------------------------------
 
+-- Axiom 1
 def MulNatZeroEqZero 
-  {P : Sort u} (L : Logic P) (N : Type v) [LEq P N] [Nat P N] [Zero N] [Mul N] :=
-  (a b : N) -> (L |- nat a) -> (L |- nat b) -> (L |- a * 0 = 0)
+  {P : Sort u} (L : Logic P) (T : Type v) [LEq P T] [Nat P T] [Zero T] [Mul T] :=
+  (a b : T) -> (L |- nat a) -> (L |- nat b) -> (L |- a * 0 = 0)
 
+-- Axiom 2
 def MulNatSuccEqAddMul 
-  {P : Sort u} (L : Logic P) (N : Type v) 
-  [LEq P N] [Nat P N] [Succ N] [Add N] [Mul N] := 
-  (a b : N) -> (L |- nat a) -> (L |- nat b) -> (L |- a + S b = a + S (a * b))
+  {P : Sort u} (L : Logic P) (T : Type v) 
+  [LEq P T] [Nat P T] [Succ T] [Add T] [Mul T] := 
+  (a b : T) -> (L |- nat a) -> (L |- nat b) -> (L |- a + S b = a + S (a * b))
 
 end Gaea.Peano.Rules
