Gaea/Logic/Basic.lean
@@ -5,11 +5,13 @@ def Logic.{u,v} (prop : Sort u)
 
 namespace Logic
 
-def prop.{u,v} {P : Sort u} (L : Logic.{u,v} P) := P
+def prop.{u,v} {P : Sort u} (L : Logic.{u,v} P) : Sort u 
+  := P
 
-def Proof.{u,v} {P : Sort u} (L : Logic.{u,v} P) := Sort v
+def Proof.{u,v} {P : Sort u} (L : Logic.{u,v} P) : Type v 
+  := Sort v
 
-def Judgment.{u,v} {P : Sort u} (L : Logic.{u,v} P) (prop : P) 
+def Judgment.{u,v} {P : Sort u} (L : Logic.{u,v} P) (prop : P) : Sort v 
   := L prop
 
 end Logic
