Gaea/Peano/Theorems.lean
@@ -6,65 +6,70 @@ import Gaea.Peano.Rules
 
 universes u v w
 
-namespace Gaea.Peano
-
 open Gaea.Syntax
 open Gaea.Logic.Rules
 open Gaea.Peano.Rules
 
+namespace Gaea.Peano
+
+--------------------------------------------------------------------------------
 -- General Theorems
+--------------------------------------------------------------------------------
 
 def natCases 
-{P : Sort u} {L : Logic P} {N : Type v} 
-[Nat P N] [Zero N] [Succ N]
-(natInduction : NatInduction L N)
-: (f : N -> P) -> 
-  (L |- f 0) -> ((n : N) -> (L |- nat n) -> (L |- f (S n))) -> 
-    ((n : N) -> (L |- nat n) -> (L |- f n))
+{P : Sort u} {L : Logic P} {T : Type v} 
+[Nat P T] [Zero T] [Succ T]
+(natInduction : NatInduction L T)
+: (f : T -> P) -> 
+  (L |- f 0) -> ((n : T) -> (L |- nat n) -> (L |- f (S n))) -> 
+    ((n : T) -> (L |- nat n) -> (L |- f n))
 := by
   intro f f0 fS n nat_n
-  have ih : (n : N) -> (L |- nat n) -> (L |- f n) -> (L |- f (S n)) := 
+  have ih : (n : T) -> (L |- nat n) -> (L |- f n) -> (L |- f (S n)) := 
     fun n nat_n fn => fS n nat_n
   exact natInduction f f0 ih n nat_n
 
+--------------------------------------------------------------------------------
 -- Addition Theorems
+--------------------------------------------------------------------------------
 
 theorem addZeroEqZero 
-{P : Sort u} {L : Logic P} {N : Type v} 
-[LEq P N] [Nat P N] [Zero N] [Add N] 
-(nat_0 : NatZero L N) 
-(An0_eq_n : AddNatZeroEqNat L N)
-: L |- 0 + 0 = (0 : N) 
+{P : Sort u} {L : Logic P} {T : Type v} 
+[LEq P T] [Nat P T] [Zero T] [Add T] 
+(nat_0 : NatZero L T) 
+(An0_eq_n : AddNatZeroEqNat L T)
+: L |- 0 + 0 = (0 : T) 
 := An0_eq_n 0 nat_0
 
 theorem natAddNatZero
-{P : Sort u} {L : Logic P} {N : Type v} 
-[LEq P N] [Nat P N] [Zero N] [Add N] 
-(natEq : NatEq L N) 
-(An0_eq_n : AddNatZeroEqNat L N)
-: (a : N) -> (L |- nat a) -> (L |- nat (a + 0))
+{P : Sort u} {L : Logic P} {T : Type v} 
+[LEq P T] [Nat P T] [Zero T] [Add T] 
+(natEq : NatEq L T) 
+(An0_eq_n : AddNatZeroEqNat L T)
+: (a : T) -> (L |- nat a) -> (L |- nat (a + 0))
 := by
   intro a nat_a
   apply natEq _ a nat_a
   exact An0_eq_n a nat_a
 
+-- Uses standard (predicate) induction
 theorem NatAddNat_induct
-{P : Sort u} {L : Logic P} {N : Type v} 
-[LForall P N] [LIf P] [LEq P N] [Nat P N] [Zero N] [Succ N] [Add N]
+{P : Sort u} {L : Logic P} {T : Type v} 
+[LForall P T] [LIf P] [LEq P T] [Nat P T] [Zero T] [Succ T] [Add T]
 (ifIntro : IfIntro L)
 (ifElim : IfElim L)
-(forallIntro : ForallIntro L N)
-(forallElim : ForallElim L N)
-(nat_S : NatSuccNat L N) 
-(natEq : NatEq L N) 
-(natInduction : NatInduction L N)
-(An0_eq_n : AddNatZeroEqNat L N)
-(AnS_eq_S : AddNatSuccEqSucc L N)
-: (b : N) -> (L |- nat b) -> (L |- forall (a : N) => nat a -> nat (a + b))
+(forallIntro : ForallIntro L T)
+(forallElim : ForallElim L T)
+(nat_S : NatSuccNat L T) 
+(natEq : NatEq L T) 
+(natInduction : NatInduction L T)
+(An0_eq_n : AddNatZeroEqNat L T)
+(AnS_eq_S : AddNatSuccEqSucc L T)
+: (b : T) -> (L |- nat b) -> (L |- forall (a : T) => nat a -> nat (a + b))
 := by
   intro b nat_b
   apply natInduction 
-    (fun b => forall (a : N) => nat a -> nat (a + b))
+    (fun b => forall (a : T) => nat a -> nat (a + b))
   -- Base
   apply forallIntro; intro a
   apply ifIntro; intro nat_a
@@ -79,19 +84,39 @@ theorem NatAddNat_induct
   exact natEq _ _ nat_SAba abSa_eq_Saba
   exact nat_b
 
+theorem NatAddNat
+{P : Sort u} {L : Logic P} {T : Type v} 
+[LForall P T] [LIf P] [LEq P T] [Nat P T] [Zero T] [Succ T] [Add T]
+(ifIntro : IfIntro L)
+(ifElim : IfElim L)
+(forallIntro : ForallIntro L T)
+(forallElim : ForallElim L T)
+(nat_S : NatSuccNat L T) 
+(natEq : NatEq L T) 
+(natInduction : NatInduction L T)
+(An0_eq_n : AddNatZeroEqNat L T)
+(AnS_eq_S : AddNatSuccEqSucc L T)
+: (a b : T) -> (L |- nat a) -> (L |- nat b) -> (L |- nat (a + b))
+:= by
+  intro a b nat_a nat_b
+  have h :=  NatAddNat_induct ifIntro ifElim forallIntro forallElim  
+    nat_S natEq natInduction An0_eq_n AnS_eq_S b nat_b
+  exact ifElim _ _ (forallElim _ h a) nat_a
+
+-- Uses schema induction
 theorem NatAddNat'
-{P : Sort u} {L : Logic.{u,w} P} {N : Type v} 
-[LEq P N] [Nat P N] [Zero N] [Succ N] [Add N]
-(nat_S : NatSuccNat L N) 
-(natEq : NatEq L N) 
-(natInduction : NatInduction'.{u,v,(imax (v+1) w)} L N)
-(An0_eq_n : AddNatZeroEqNat L N)
-(AnS_eq_S : AddNatSuccEqSucc L N)
-: (a b : N) -> (L |- nat a) -> (L |- nat b) -> (L |- nat (a + b))
+{P : Sort u} {L : Logic.{u,w} P} {T : Type v} 
+[LEq P T] [Nat P T] [Zero T] [Succ T] [Add T]
+(nat_S : NatSuccNat L T) 
+(natEq : NatEq L T) 
+(natInduction : NatInduction'.{u,v,(imax (v+1) w)} L T)
+(An0_eq_n : AddNatZeroEqNat L T)
+(AnS_eq_S : AddNatSuccEqSucc L T)
+: (a b : T) -> (L |- nat a) -> (L |- nat b) -> (L |- nat (a + b))
 := by
   intro m n nat_m nat_n
   apply natInduction
-    (fun b => (a : N) -> (L |- nat a) -> (L |- nat (a + b)))
+    (fun b => (a : T) -> (L |- nat a) -> (L |- nat (a + b)))
   -- Base
   intro a nat_a
   exact natAddNatZero natEq An0_eq_n a nat_a
@@ -102,24 +127,5 @@ theorem NatAddNat'
   have nat_SAba := nat_S _ nat_Aba
   exact natEq _ _ nat_SAba abSa_eq_Saba
   exact nat_n; exact nat_m
-
-theorem NatAddNat
-{P : Sort u} {L : Logic P} {N : Type v} 
-[LForall P N] [LIf P] [LEq P N] [Nat P N] [Zero N] [Succ N] [Add N]
-(ifIntro : IfIntro L)
-(ifElim : IfElim L)
-(forallIntro : ForallIntro L N)
-(forallElim : ForallElim L N)
-(nat_S : NatSuccNat L N) 
-(natEq : NatEq L N) 
-(natInduction : NatInduction L N)
-(An0_eq_n : AddNatZeroEqNat L N)
-(AnS_eq_S : AddNatSuccEqSucc L N)
-: (a b : N) -> (L |- nat a) -> (L |- nat b) -> (L |- nat (a + b))
-:= by
-  intro a b nat_a nat_b
-  have h :=  NatAddNat_induct ifIntro ifElim forallIntro forallElim  
-    nat_S natEq natInduction An0_eq_n AnS_eq_S b nat_b
-  exact ifElim _ _ (forallElim _ h a) nat_a
 
 end Gaea.Peano
